fix: Encrypt/DecryptInput updates

src/Generated/AwsEncryptionSdk.dfy
@@ -14,38 +14,25 @@ module {:extern "Dafny.Aws.Esdk"} Aws.Esdk {
     datatype EncryptInput = EncryptInput(
         nameonly plaintext: seq<uint8>,
         nameonly encryptionContext: Crypto.EncryptionContext, // TODO Make an option?
-        nameonly materialsManager: Crypto.ICryptographicMaterialsManager,
-        nameonly algorithmSuiteId: Option<Crypto.AlgorithmSuiteId>
-        // TODO reintroduce optional materialsManager and optional keyring
+        nameonly materialsManager: Crypto.ICryptographicMaterialsManager?,
+        nameonly keyring: Crypto.IKeyring?,
+        nameonly algorithmSuiteId: Option<Crypto.AlgorithmSuiteId>,
+        nameonly plaintextLength: nat, // TODO add to smithy model, or remove from encrypt logic
+        nameonly frameLength: Option<uint32> // TODO add to smithy model, or remove from encrypt logic
     )
-    {
-        predicate Valid() {
-            true 
-        }
-    }
 
     datatype EncryptOutput = EncryptOutput(
-        nameonly ciphertext: seq<uint8>
+        nameonly encryptedMessage: seq<uint8> // TODO update smithy model name
         // TODO Hook up additional Encryption outputs
         // nameonly encryptionContext: Crypto.EncryptionContext,
         // nameonly algorithmSuiteId: Crypto.AlgorithmSuiteId
     )
-    {
-        predicate Valid() {
-            true 
-        }
-    }
 
     datatype DecryptInput = DecryptInput(
-        nameonly ciphertext: seq<uint8>,
-        nameonly materialsManager: Crypto.ICryptographicMaterialsManager
-        // TODO reintroduce optional and keyring
+        nameonly encryptedMessage: seq<uint8>, // TODO update smithy model name
+        nameonly materialsManager: Crypto.ICryptographicMaterialsManager?,
+        nameonly keyring: Crypto.IKeyring?
     )
-    {
-        predicate Valid() {
-            true 
-        }
-    }
 
     datatype DecryptOutput = DecryptOutput(
         nameonly plaintext: seq<uint8>
@@ -53,28 +40,16 @@ module {:extern "Dafny.Aws.Esdk"} Aws.Esdk {
         // nameonly encryptionContext: Crypto.EncryptionContext,
         // nameonly algorithmSuiteId: Crypto.AlgorithmSuiteId
     )
-    {
-        predicate Valid() {
-            true 
-        }
-    }
 
     // datatype AwsEncryptionSdkClientConfig = AwsEncryptionSdkClientConfig(
     //     nameonly commitmentPolicy: string,
     //     nameonly maxEncryptedEdks: int,
     //     nameonly configDefaults: ConfigurationDefaults
     // )
-    // {
-    //     predicate Valid() {
-    //         true
-    //     }
-    // }
 
     trait {:termination false} IAwsEncryptionSdkClient {
         method Encrypt(input: EncryptInput) returns (res: Result<EncryptOutput, string>)
-            requires input.Valid()
         method Decrypt(input: DecryptInput) returns (res: Result<DecryptOutput, string>)
-            requires input.Valid()
         // TODO I can't seem to find a way to get this to work
         // static method {:extern "createClient"} createClient(clientConfig: AwsEncryptionSdkClientConfig) returns (res: IAwsEncryptionSdkClient)
     }
