src/SDK/AwsEncryptionSdk.dfy
@@ -24,17 +24,13 @@ module {:extern "Dafny.Aws.Esdk.AwsEncryptionSdkClient"} AwsEncryptionSdk {
         constructor () {}
 
         method Encrypt(input: Esdk.EncryptInput) returns (res: Result<Esdk.EncryptOutput, string>)
-            requires input.Valid()
         {
-            var encryptRequest := EncryptDecrypt.EncryptRequest.WithCMM(input.plaintext, input.materialsManager).SetEncryptionContext(input.encryptionContext);
-            var e :- expect EncryptDecrypt.Encrypt(encryptRequest);
-            return Success(Esdk.EncryptOutput(ciphertext:=e));
+            var e :- expect EncryptDecrypt.Encrypt(input);
+            return Success(Esdk.EncryptOutput(encryptedMessage:=e));
         }
         method Decrypt(input: Esdk.DecryptInput) returns (res: Result<Esdk.DecryptOutput, string>)
-            requires input.Valid()
         {
-            var decryptRequest := EncryptDecrypt.DecryptRequest.WithCMM(input.ciphertext, input.materialsManager);
-            var d :- expect EncryptDecrypt.Decrypt(decryptRequest);
+            var d :- expect EncryptDecrypt.Decrypt(input);
             return Success(Esdk.DecryptOutput(plaintext:=d));
         }
   }
